rkt/unravel.rkt
@@ -1,0 +1,16 @@
+#lang at-exp s-exp "tmonad.rkt"
+
+(provide unravel)
+
+(Fixpoint
+ unravel #:implicit @A{Set} @xs{list A}
+ #:returns @{list A * list A}
+ (match (xs)
+   [(nil) => (<== (pair nil nil))]
+   [(cons x xs′)
+    =>
+    (bind ([odds_evens (unravel xs′)])
+          (match (odds_evens)
+            [(pair odds evens)
+             =>
+             (<== (pair (cons x evens) odds))]))]))
