make_array/make_array_nlogn2.v
@@ -8,59 +8,101 @@ Require Import Braun.common.array.
 Require Import Braun.common.util.
 Require Import Braun.common.log.
 
-Program Fixpoint unravel (A:Set) (xs:list A) :
-  {! eo !:! ((list A) * (list A))
-     !<! c !>!
-     let (e, o) := eo in
-     xs = interleave e o 
-     /\ length o <= length e <= length o + 1
-     /\ c = length xs !} :=
-  match xs with
-    | nil =>
-      <== (nil, nil)
-    | (cons x xs') =>
-      moe <- unravel A xs' ;
-      ++ ;
-      <== ( (cons x (snd moe)), (fst moe) )
-  end.
+Require Import Braun.common.big_oh Braun.common.le_util Braun.common.util.
+
+Require Import Arith Arith.Even Arith.Div2 Omega.
+Require Import Program.Wf Init.Wf.
+
+Include WfExtensionality.
+
+Definition unravel_time len := 10 * len + 5.
+
+Definition unravel_result (A:Set) (xs:list A) (eo:list A * list A) (c:nat) :=
+  let (e, o) := eo in
+  xs = interleave e o 
+  /\ length o <= length e <= length o + 1
+  /\ c = unravel_time (length xs).
+
+Load "unravel_gen.v".
 
 Next Obligation.
-  simpl.
+Proof.
   rewrite interleave_case2.
-  split. auto. omega.
+  split; auto.
+  split.
+  omega.
+  unfold unravel_time.
+  omega.
 Qed.
 
-Program Fixpoint make_array_td (A:Set) xs {measure (length xs)} :
-  {! b !:! @bin_tree A
-     !<! c !>!
-     let n := length xs in
-     Braun b n
-     /\ c = mat_time n
-     /\ SequenceR b xs !} :=
-  match xs with
-    | nil      =>
-      <== bt_mt
-    | (cons x xs') =>
-      eo <- unravel A xs' ;
-      oa <- make_array_td A (fst eo) ;
-      ea <- make_array_td A (snd eo) ;
-      ++ ; 
-      <== (bt_node x oa ea)
+Program Fixpoint make_array_td_time n {measure n} :=
+  match n with
+    | 0 => 3
+    | S n' => 
+      10 * n' + 18 + 
+      make_array_td_time (div2 (n'+1)) +
+      make_array_td_time (div2 n')
   end.
+Next Obligation.
+Proof.
+  replace (n'+1) with (S n').
+  auto.
+  omega.
+Qed.
+
+Definition make_array_td_result (A:Set) xs (b:@bin_tree A) c :=
+  let n := length xs in
+  Braun b n
+  /\ c = make_array_td_time n
+  /\ SequenceR b xs.
+
+Load "make_array_nlogn2_gen.v".
 
 Next Obligation.
+Proof.
+  repeat split; auto.
+Qed.
+
+Next Obligation.
+Proof.
+  clear make_array_td.
+  rename H into UR.
+
+  unfold unravel_result in UR.
+  destruct UR.
+  subst xs'.
   simpl. rewrite <- interleave_length_split.
   omega.
 Qed.
 
 Next Obligation.
+Proof.
+  clear make_array_td.
+  clear H am0.
+  rename H0 into UR.
+  unfold unravel_result in UR.
+  destruct UR.
+  subst xs'.
   simpl. rewrite <- interleave_length_split.
   omega.
 Qed.
  
 Next Obligation.
-  simpl in *.
+Proof.
+  clear make_array_td.
+  clear am1 H6.
+  clear am0 H7.
+  rename H0 into MATRevens.
+  rename H1 into MATRodds.
   rename l into e. rename l0 into o.
+
+  unfold unravel_result in *.
+  unfold make_array_td_result in *.
+  
+  destruct MATRevens as [BRevens [ANeq SEQevens]].
+  destruct MATRodds as [BRodds [AN0eq SEQodds]].
+
+  simpl in *.
   rewrite <- interleave_length_split.
   split; [|split].
 
@@ -69,8 +111,76 @@ Next Obligation.
   eauto.
 
   (* running time *)
-  rewrite <- braun_implies_mat_time; omega.
+  remember (length e) as LE; clear HeqLE.
+  remember (length o) as LO; clear HeqLO.
+  subst an0 an.
+  unfold unravel_time.
+  assert (LE = LO \/ LE = LO + 1) as TWOCASES; try omega.
+  destruct TWOCASES; subst LE; clear.
+  unfold_sub make_array_td_time (make_array_td_time (S (LO+LO))).
+  replace (div2 (LO+LO)) with LO; [|rewrite double_div2; reflexivity].
+  replace (div2 (LO+LO+1)) with LO.
+  omega.
+  rewrite <- (div2_with_odd_argument LO) at 1.
+  replace (LO+LO+1) with (S (LO+LO)); omega.
+
+  unfold_sub make_array_td_time (make_array_td_time (S (LO+1+LO))).
+  replace (LO+1+LO+1) with ((LO+1)+(LO+1)); try omega.
+  replace (div2 ((LO+1)+(LO+1))) with (LO+1);[|rewrite double_div2; reflexivity].
+  replace (div2 (LO+1+LO)) with LO.
+  omega.
+  rewrite <- (div2_with_odd_argument LO) at 1.
+  replace (LO+1+LO) with (S (LO+LO)); omega.
 
   (* correctness *)
   eauto.
+Qed.
+
+Theorem make_array_td_nlogn : big_oh make_array_td_time (fun n => n*fl_log n).
+Proof.
+  exists 1.
+  exists 50.
+  intros n LT.
+  destruct n;intuition.
+  clear LT.
+  apply (well_founded_induction
+           lt_wf
+           (fun n =>  make_array_td_time (S n) <= 50 * (S n * fl_log (S n)))).
+  clear n; intros n IND.
+  destruct n.
+  compute.
+  omega.
+  destruct n.
+  compute.
+  omega.
+  remember (S (S n)) as m.
+  unfold_sub make_array_td_time (make_array_td_time (S m)).
+  subst m.
+  replace (S (S n) + 1) with (S (S (S n))); try omega.
+  replace (div2 (S (S (S n)))) with (S (div2 (S n)));[|simpl;reflexivity].
+  replace (div2 (S (S n))) with (S (div2 n));[|simpl;reflexivity].
+  apply (le_trans (10 * S (S n) + 18 +
+                   make_array_td_time (S (div2 (S n))) +
+                   make_array_td_time (S (div2 n)))
+                  (10 * S (S n) + 18 +
+                   make_array_td_time (S (div2 (S n))) +
+                   (50 * (S (div2 n) * fl_log (S (div2 n)))))
+                  (50 * (S (S (S n)) * fl_log (S (S (S n)))))).
+  apply le_plus_right.
+  apply IND.
+  apply (lt_trans (div2 n) (S n) (S (S n))); auto.
+  apply (le_trans (10 * S (S n) + 18 +
+                   make_array_td_time (S (div2 (S n))) +
+                   (50 * (S (div2 n) * fl_log (S (div2 n)))))
+                  (10 * S (S n) + 18 +
+                   (50 * (S (div2 (S n)) * fl_log (S (div2 (S n))))) +
+                   (50 * (S (div2 n) * fl_log (S (div2 n)))))
+                  (50 * (S (S (S n)) * fl_log (S (S (S n)))))).
+  apply le_plus_left.
+  apply le_plus_right.
+  apply IND;auto.
+
+  clear IND.
+  
+  admit. (* might be true .... *)
 Qed.
