README.md
@@ -16,7 +16,7 @@ Volume 7 Issue 6, November 1997, 661 - 666
 
 TODO:
 - size_diff (redo with Racket generation, big_oh)   [robby]
-- make_array_td (redo with Racket generation, big_oh) [robby]
+- make_array_td (big_oh) [robby]
 - make_array_bu (time, correctness, extraction, big_oh) [max]
 - to_list_naive (exact time [vs bound], big_oh)
 - to_list_bu (time, correctness, extraction, big_oh)
